Qed durable message passing example

src/examples/durable_mp.v
@@ -1,4 +1,6 @@
 From iris.proofmode Require Import tactics.
+From iris.algebra Require Import excl.
+From Perennial.program_logic Require Import staged_invariant.
 
 From self.base Require Import primitive_laws.
 From self.lang Require Import lang.
@@ -35,12 +37,13 @@ Section program.
 End program.
 
 Section proof.
-  Context `{nvmFixedG Σ, nvmDeltaG Σ}.
+  Context `{nvmFixedG Σ, nvmDeltaG Σ, inG Σ (exclR unitO)}.
+  Context `{!stagedG Σ}.
 
-  Context (x y z : loc).
+  Context (x y z : loc) (γ__ex : gname).
 
   Definition inv_x (b : bool) (v : val) (hG : nvmDeltaG Σ) : dProp Σ :=
-    ⌜v = #(Nat.b2n b)⌝.
+    ⌜v = #b⌝.
 
   Program Instance : LocationProtocol inv_x := { bumper n := n }.
   Next Obligation. iIntros. by iApply post_crash_flush_pure. Qed.
@@ -48,7 +51,7 @@ Section proof.
 
   Definition inv_y (b : bool) (v : val) (hG : nvmDeltaG Σ) : dProp Σ :=
     match b with
-      false => ⌜ v = #false ⌝
+      false => ⌜ v = #false ⌝ ∗ ⎡ own γ__ex (Excl ()) ⎤
     | true => ⌜ v = #true ⌝ ∗ know_flush_lb x true
     end.
 
@@ -59,15 +62,13 @@ Section proof.
       iDestruct "lb" as "(% & %le & h & hi & _)".
       destruct s__pc; last done.
       iFrame "∗%".
-    - iIntros "%". iApply post_crash_flush_pure. done.
+    - iIntros "[% H]". iCrashFlush. iFrame. done.
   Qed.
   Next Obligation.
     rewrite /inv_y. iIntros (???) "H". iModIntro. done.
   Qed.
 
   Definition inv_z := inv_y.
-  (* Definition inv_z (b : bool) (v : val) (hG : nvmDeltaG Σ) : dProp Σ := *)
-  (*   ⌜v = #(Nat.b2n b)⌝ ∗ (⌜b = true⌝ -∗ know_flush_lb x true). *)
 
   Definition crash_condition {hD : nvmDeltaG Σ} : dProp Σ :=
     ∃ (sx sz : list bool),
@@ -85,22 +86,12 @@ Section proof.
       "#zProt" ∷ know_protocol z inv_z ∗
       z ↦ₚ sz.
 
-  (* Lemma crash_condition_impl {hD : nvmDeltaG Σ} (ssX ssZ : list bool) : *)
-  (*   know_protocol x inv_x -∗ know_protocol y inv_y -∗ know_protocol z inv_z -∗ *)
-  (*   x ↦ₚ ssX -∗ *)
-  (*   ⎡ is_shared_loc y ⎤ -∗ *)
-  (*   z ↦ₚ ssZ -∗ *)
-  (*   <PC> hG, crash_condition. *)
-  (* Proof. *)
-  (*   iIntros "xPred yProt zProt xPts yShared zPts". *)
-  (*   iCrash. *)
-  (*   iDestruct "xPts" as (??) "[xPts xRec]". *)
-  (*   iDestruct "zPts" as (??) "[zPts zRec]". *)
-  (*   iExists _, _. *)
-  (*   iDestruct (recovered_at_or_lost with "xRec xPred") as "xPred". *)
-  (*   iDestruct (recovered_at_or_lost with "zRec zProt") as "zProt". *)
-  (*   iFrame. *)
-  (* Qed. *)
+  Definition left_crash_condition {hD : nvmDeltaG Σ} : dProp Σ :=
+    ∃ (sx : list bool),
+      "#yProt" ∷ or_lost y (know_protocol y inv_y) ∗
+      "#yShared" ∷ or_lost y (⎡ is_shared_loc y ⎤) ∗
+      "#xProt" ∷ know_protocol x inv_x ∗
+      x ↦ₚ sx.
 
   Lemma right_crash_condition_impl {hD : nvmDeltaG Σ} (ssZ : list bool) :
     know_protocol y inv_y -∗
@@ -118,10 +109,30 @@ Section proof.
     iFrame.
   Qed.
 
+  Lemma left_crash_condition_impl {hD : nvmDeltaG Σ} (ssX : list bool) :
+    know_protocol y inv_y -∗
+    know_protocol x inv_x -∗
+    know_store_lb y false -∗
+    ⎡ is_shared_loc y ⎤ -∗
+    x ↦ₚ ssX -∗
+    <PC> hD, left_crash_condition.
+  Proof.
+    iIntros "yProt xProt yLb yShared xPts".
+    iCrash.
+    iDestruct "xPts" as (??) "[xPts xRec]".
+    iExists _.
+    iDestruct (recovered_at_or_lost with "xRec xProt") as "xProt".
+    iFrame.
+  Qed.
+
   (* Prove right crash condition. *)
   Ltac whack_right_cc :=
     iSplit;
     first iApply (right_crash_condition_impl with "yProt zProt yLb yShared zPts").
+
+  Ltac whack_left_cc :=
+    iSplit;
+    first iApply (left_crash_condition_impl with "yProt xProt yLb yShared xPts").
 
   Lemma right_prog_spec s k E1 :
     know_protocol y inv_y -∗
@@ -142,7 +153,7 @@ Section proof.
     { iModIntro. iIntros (?? incl) "a". rewrite /inv_y.
       destruct s'.
       - iDestruct "a" as "[% #?]". iFrame "#". naive_solver.
-      - iDestruct "a" as "%". naive_solver. }
+      - iDestruct "a" as "[% O]". naive_solver. }
     iNext.
     iIntros (??) "[yLb' disj]".
     iDestruct (post_fence_extract' _ (⌜v = #true ∨ v = #false⌝)%I with "disj []") as %[-> | ->].
@@ -195,12 +206,12 @@ Section proof.
     {{ <PC> _, crash_condition }}.
   Proof.
     iIntros "(pb & #xProt & #yProt & #zProt & xPts & #yLb & #yShared & zPts)".
-    (* iIntros "H". *)
     rewrite /prog.
 
     (* We create a crash borrow in order to transfer resources to the forked
     thread. *)
-    iApply (wpc_crash_borrow_inits _ _ _ _ _ _ (<PC> _, right_crash_condition)%I with "pb [zPts]").
+    iApply (wpc_crash_borrow_inits _ _ _ _ _ _ (<PC> _, right_crash_condition)%I
+             with "pb [zPts]").
     { iAccu. }
     { iModIntro. iIntros "zPts".
       iDestruct "zProt" as "-#zProt".
@@ -212,9 +223,18 @@ Section proof.
       iExists _. iFrame. }
     iIntros "cb".
 
+    iApply (wpc_crash_mono _ _ _ _ _ _ (<PC> _, left_crash_condition)%I).
+    { iIntros "L R".
+      iCrash.
+      iDestruct "L"  as (?) "(H1 & H2 & H3 & xPts)".
+      iDestruct "R" as (?) "(? & ? & ? & ?)".
+      iExists _, _.
+      iFrame. }
+    Unshelve. 2: { apply _. }
+
     wpc_bind (Fork _)%E.
     iApply (wpc_fork with "[cb]").
-    { (* Show safety of the forked off thread. *)
+    - (* Show safety of the forked off thread. *)
       iApply (wpc_crash_borrow_open_modify with "cb"); first done.
       iNext. iSplit; first done.
       iIntros "zPts". rewrite (left_id True%I (∗)%I).
@@ -222,16 +242,68 @@ Section proof.
       iDestruct (right_prog_spec with "yProt zProt yLb yShared zPts") as "wp".
       iApply (wpc_mono' with "[] [] wp"); last naive_solver.
       iIntros (?) "[zPts | zPts]".
-      - iExists (z ↦ₚ (_ : list bool)). iFrame.
+      * iExists (z ↦ₚ (_ : list bool)). iFrame.
         iSplit; last naive_solver.
         iIntros "!> zPts".
         iApply (right_crash_condition_impl with "yProt zProt yLb yShared zPts").
-      - iExists (z ↦ₚ (_ : list bool)). iFrame.
+      * iExists (z ↦ₚ (_ : list bool)). iFrame.
         iSplit; last naive_solver.
         iIntros "!> zPts".
         iApply (right_crash_condition_impl with "yProt zProt yLb yShared zPts").
-    }
-    { admit. }
-  Abort.
+    - whack_left_cc. iNext.
+      wpc_pures.
+      { iApply (left_crash_condition_impl with "yProt xProt yLb yShared xPts"). }
+      rewrite /leftProg.
+      wpc_bind (_ <- _)%E.
+      iApply wpc_atomic_no_mask. whack_left_cc.
+      iApply (wp_store_ex x _ _ _ _ true with "[$xProt $xPts]").
+      { reflexivity. } { done. }
+      { rewrite /inv_x. done. }
+      simpl.
+      iNext. iIntros "xPts".
+      whack_left_cc.
+      iModIntro.
+      wpc_pures;
+      first iApply (left_crash_condition_impl with "yProt xProt yLb yShared xPts").
+
+      (* WB *)
+      wpc_bind (WB _)%E.
+      iApply wpc_atomic_no_mask.
+      whack_left_cc.
+      iApply (wp_wb_ex with "xPts"); first reflexivity.
+      iNext.
+      iIntros "[xPts afterFence]".
+      whack_left_cc.
+      iModIntro.
+      wpc_pures;
+      first iApply (left_crash_condition_impl with "yProt xProt yLb yShared xPts").
+
+      (* The fence. *)
+      wpc_bind (Fence)%E.
+      iApply wpc_atomic_no_mask. whack_left_cc.
+      iApply (wp_fence with "afterFence").
+      iNext.
+      iIntros "#xLowerBound".
+      whack_left_cc.
+      iModIntro.
+      wpc_pures;
+      first iApply (left_crash_condition_impl with "yProt xProt yLb yShared xPts").
+
+      wpc_bind (_ <-{rel} _)%E.
+      iApply wpc_atomic_no_mask. whack_left_cc.
+      iApply (wp_store_at _ false true).
+      { iFrame.
+        iPureGoal. { done. }
+        iFrame "#".
+        iSplitL.
+        - iModIntro. simpl. naive_solver.
+        - iIntros (? s_c v_c). simpl.
+          destruct s_c; first naive_solver.
+          iIntros "([? O1] & [??] & [? O2])".
+          by iDestruct (own_valid_2 with "O1 O2") as %HI%exclusive_l. }
+      iIntros "!> yLb2".
+      whack_left_cc.
+      done.
+  Qed.
 
 End proof.
